\section{Correctness of Horner's rule}

\subsection{a}

The running time is $\Theta(n)$.


\subsection{b}

\yin{Naive-Polynomial-Evaluation} shows the pseudocode of naive polynomial-evaluation algorithm.
The running time is $\Theta(n^2)$.

\begin{codebox}
\Procname{$\proc{Naive-Polynomial-Evaluation}(P(x), x)$}
\li	$\id{y} \gets 0$
\li	\For $i \gets 0$ \To $n$
\li	\Do
		$\id{t} \gets 1$
\li		\For $j \gets 1$ \To $i$
\li		\Do
			$\id{t} \gets \id{t} \cdot x$
		\End
\li		$\id{y} \gets \id{y} + \id{t} \cdot a_i$
	\End
\li	\Return $\id{y}$
\end{codebox}


\subsection{c}

\paragraph{Initialization}
Prior to the first iteration of the loop, we have $i = n$, so that $\sum_{k = 0}^{n - (i + 1)} a_{k + i + 1} x^k = \sum_{k = 0}^{-1} a_{k + n + 1} = 0$ consistent with $k = 0$. So loop invariant holds.

\paragraph{Maintenance}
By loop invariant, we have $y = \sum_{k = 0}^{n - (i + 1)} a_{k + i + 1} x^k$.
Then lines 2-3 perform that

\begin{equation}\notag
\begin{aligned}
y' &= a_i + x \cdot y\\
&= a_i + x \cdot (\sum_{k = 0}^{n - (i + 1)} a_{k + i + 1} x^k)\\
&= a_i + \sum_{k = 0}^{n - (i + 1)} a_{k + i + 1} x^{k + 1}\\
&= \sum_{k = 0}^{n - i} a_{k + i} x^k
\end{aligned}
\end{equation}

So decrementing $i$ reestablishes the loop invariant for the next iteration.

\paragraph{Termination}
At termination, $i = -1$. By loop invariant, we get the result $y = \sum_{k = 0}^n a_k x^k$.


\subsection{d}

The given code fragment correctly evaluates a polynomial characterized by the coefficients $a_0, a_1, \cdots, a_n$, i.e.

\begin{equation}\notag
y = \sum_{k = 0}^n a_k x^k = P(x)
\end{equation}